src/program_proof/tulip/paxos/invariance/advance.v
@@ -22,17 +22,21 @@ Qed.
 Section advance.
   Context `{!paxos_ghostG Σ}.
 
-  Lemma node_inv_advance {γ nids nid termc terml lsnc v} v' :
+  Lemma node_inv_advance {γ nids nid wal termc terml lsnc v} ents v' :
     (terml < termc)%nat ->
+    (lsnc ≤ length v)%nat ->
+    ents = drop lsnc v' ->
     (lsnc ≤ length v')%nat ->
     prefix (take lsnc v) v' ->
     prefix_base_ledger γ termc v' -∗
     prefix_growing_ledger γ termc v' -∗
+    own_node_wal_half γ nid wal -∗
     own_current_term_half γ nid termc -∗
     own_ledger_term_half γ nid terml -∗
     own_committed_lsn_half γ nid lsnc -∗
     own_node_ledger_half γ nid v -∗
     node_inv γ nids nid terml ==∗
+    own_node_wal_half γ nid (wal ++ [CmdPaxosAdvance termc lsnc ents]) ∗
     own_current_term_half γ nid termc ∗
     own_ledger_term_half γ nid termc ∗
     own_committed_lsn_half γ nid lsnc ∗
@@ -40,12 +44,16 @@ Section advance.
     node_inv γ nids nid termc ∗
     is_accepted_proposal_lb γ nid termc v'.
   Proof.
-    iIntros (Hlt Hlsncub Hprefix) "#Hpfb #Hpfg HtermcX HtermlX HlsncX HlognX Hinv".
+    iIntros (Hlt Hlenv Hents Hlsncub Hprefix) "#Hpfb #Hpfg HwalX HtermcX HtermlX HlsncX HlognX Hinv".
     iNamed "Hinv".
     (* Agreements on the current term, committed LSN, and the node ledger. *)
+    iDestruct (node_wal_agree with "HwalX Hwalnode") as %->.
     iDestruct (current_term_agree with "HtermcX Htermc") as %->.
     iDestruct (committed_lsn_agree with "HlsncX Hlsnc") as %->.
     iDestruct (node_ledger_agree with "HlognX Hlogn") as %->.
+    (* Update the write-ahead log. *)
+    set wal' := wal ++ _.
+    iMod (node_wal_update wal' with "HwalX Hwalnode") as "[HwalX Hwalnode]".
     (* Update the ledger term to [termc]. *)
     iMod (ledger_term_update termc with "HtermlX Hterml") as "[HtermlX Hterml]".
     (* Update the current ledger to [v']. *)
@@ -88,21 +96,36 @@ Section advance.
       assert (Hne : t ≠ termc) by lia.
       set_solver.
     }
-    done.
+    split; first done.
+    { rewrite /execute_paxos_cmds foldl_snoc /= /execute_paxos_advance.
+      rewrite execute_paxos_cmds_unfold Hexec.
+      case_decide; last lia.
+      f_equal.
+      rewrite Hents -{2}(take_drop lsnc v').
+      f_equal.
+      destruct Hprefix as [l ->].
+      rewrite take_app_le; last first.
+      { rewrite length_take. clear -Hlenv. lia. }
+      by rewrite take_idemp.
+    }
   Qed.
 
-  Lemma paxos_inv_advance γ nids nid termc terml lsnc v v' :
+  Lemma paxos_inv_advance {γ nids nid wal termc terml lsnc v} ents v' :
     nid ∈ nids ->
     (terml < termc)%nat ->
+    (lsnc ≤ length v)%nat ->
+    ents = drop lsnc v' ->
     (lsnc ≤ length v')%nat ->
     prefix (take lsnc v) v' ->
     prefix_base_ledger γ termc v' -∗
     prefix_growing_ledger γ termc v' -∗
+    own_node_wal_half γ nid wal -∗
     own_current_term_half γ nid termc -∗
     own_ledger_term_half γ nid terml -∗
     own_committed_lsn_half γ nid lsnc -∗
     own_node_ledger_half γ nid v -∗
     paxos_inv γ nids ==∗
+    own_node_wal_half γ nid (wal ++ [CmdPaxosAdvance termc lsnc ents]) ∗
     own_current_term_half γ nid termc ∗
     own_ledger_term_half γ nid termc ∗
     own_committed_lsn_half γ nid lsnc ∗
@@ -110,7 +133,7 @@ Section advance.
     paxos_inv γ nids ∗
     is_accepted_proposal_lb γ nid termc v'.
   Proof.
-    iIntros (Hnid Hlt Hlsncub Hprefix) "#Hpfb #Hpfg Htermc Hterml Hlsnc Hlogn Hinv".
+    iIntros (Hnid Hlt Hlenv Hents Hlsncub Hprefix) "#Hpfb #Hpfg Hwal Htermc Hterml Hlsnc Hlogn Hinv".
     iNamed "Hinv".
     pose proof Hnid as Hterml.
     rewrite -Hdomtermlm elem_of_dom in Hterml.
@@ -118,9 +141,11 @@ Section advance.
     iDestruct (big_sepM_delete _ _ nid with "Hnodes") as "[Hnode Hnodes]".
     { apply Hterml. }
     iDestruct (own_ledger_term_node_inv_terml_eq with "Hterml Hnode") as %->.
-    iMod (node_inv_advance v' with "Hpfb Hpfg Htermc Hterml Hlsnc Hlogn Hnode")
-      as "(Htermc & Hterml & Hlsnc & Hlogn & Hnode & #Hacptlb)".
+    iMod (node_inv_advance ents v' with "Hpfb Hpfg Hwal Htermc Hterml Hlsnc Hlogn Hnode")
+      as "(Hwal & Htermc & Hterml & Hlsnc & Hlogn & Hnode & #Hacptlb)".
     { apply Hlt. }
+    { apply Hlenv. }
+    { apply Hents. }
     { apply Hlsncub. }
     { apply Hprefix. }
     iDestruct (big_sepM_insert_2 with "Hnode Hnodes") as "Hnodes".
