src/program_proof/tulip/paxos/recovery.v
@@ -1,0 +1,113 @@
+From Perennial.program_proof Require Import grove_prelude.
+From Perennial.program_proof.tulip.paxos Require Import base.
+
+Inductive pxst :=
+| PaxosState (termc terml lsnc : nat) (ledger : ledger)
+| PaxosStuck.
+
+Inductive pxcmd :=
+| CmdPaxosExtend (ents : ledger)
+| CmdPaxosAppend (ent : string)
+| CmdPaxosPrepare (term : nat)
+| CmdPaxosAdvance (term lsn : nat) (ents : ledger)
+| CmdPaxosAccept (lsn : nat) (ents : ledger)
+| CmdPaxosExpand (lsn : nat).
+
+Definition execute_paxos_extend st ents :=
+  match st with
+  | PaxosState termc terml lsnc ledger =>
+      PaxosState termc terml lsnc (ledger ++ ents)
+  | PaxosStuck => PaxosStuck
+  end.
+
+Definition execute_paxos_append st ent :=
+  match st with
+  | PaxosState termc terml lsnc ledger =>
+      PaxosState termc terml lsnc (ledger ++ [ent])
+  | PaxosStuck => PaxosStuck
+  end.
+
+Definition execute_paxos_prepare st term :=
+  match st with
+  | PaxosState termc terml lsnc ledger =>
+      PaxosState term terml lsnc ledger
+  | PaxosStuck => PaxosStuck
+  end.
+
+Definition execute_paxos_advance st term lsn ents :=
+  match st with
+  | PaxosState termc terml lsnc ledger =>
+      if decide (lsn ≤ length ledger)%nat
+      then PaxosState termc term lsnc (take lsn ledger ++ ents)
+      else PaxosStuck
+  | PaxosStuck => PaxosStuck
+  end.
+
+Definition execute_paxos_accept st lsn ents :=
+  match st with
+  | PaxosState termc terml lsnc ledger =>
+      if decide (lsn ≤ length ledger)%nat
+      then PaxosState termc terml lsnc (take lsn ledger ++ ents)
+      else PaxosStuck
+  | PaxosStuck => PaxosStuck
+  end.
+
+Definition execute_paxos_expand st lsn :=
+  match st with
+  | PaxosState termc terml lsnc ledger =>
+      PaxosState termc terml lsn ledger
+  | PaxosStuck => PaxosStuck
+  end.
+
+Definition execute_paxos_cmd st c :=
+  match c with
+  | CmdPaxosExtend ents => execute_paxos_extend st ents
+  | CmdPaxosAppend ent => execute_paxos_append st ent
+  | CmdPaxosPrepare term => execute_paxos_prepare st term
+  | CmdPaxosAdvance term lsn ents => execute_paxos_advance st term lsn ents
+  | CmdPaxosAccept lsn ents => execute_paxos_accept st lsn ents
+  | CmdPaxosExpand lsn => execute_paxos_expand st lsn
+  end.
+
+Definition init_pxst := PaxosState O O O [].
+
+Definition execute_paxos_cmds cmds :=
+  foldl execute_paxos_cmd init_pxst cmds.
+
+Lemma execute_paxos_cmds_unfold cmds :
+  foldl execute_paxos_cmd init_pxst cmds = execute_paxos_cmds cmds.
+Proof. done. Qed.
+
+Definition encode_paxos_extend (ents : ledger) : list u8.
+Admitted.
+
+Definition encode_paxos_append (ent : string) : list u8.
+Admitted.
+
+Definition encode_paxos_prepare (term : u64) : list u8.
+Admitted.
+
+Definition encode_paxos_advance (term lsn : u64) (ents : ledger) : list u8.
+Admitted.
+
+Definition encode_paxos_accept (lsn : u64) (ents : ledger) : list u8.
+Admitted.
+
+Definition encode_paxos_expand (lsn : u64) : list u8.
+Admitted.
+
+Definition encode_paxos_cmd c :=
+  match c with
+  | CmdPaxosExtend ents => encode_paxos_extend ents
+  | CmdPaxosAppend ent => encode_paxos_append ent
+  | CmdPaxosPrepare term => encode_paxos_prepare term
+  | CmdPaxosAdvance term lsn ents => encode_paxos_advance term lsn ents
+  | CmdPaxosAccept lsn ents => encode_paxos_accept lsn ents
+  | CmdPaxosExpand lsn => encode_paxos_expand lsn
+  end.
+
+Definition encode_paxos_cmds_step p c :=
+  p ++ encode_paxos_cmd c.
+
+Definition encode_paxos_cmds cmds :=
+  foldl encode_paxos_cmds_step [] cmds.
